src/tls/UntrustedCert.fst
@@ -9,78 +9,82 @@ open Platform.Error
 open TLSError
 open TLSConstants
 
-val oid_RSAEncryption : string
+
+abstract val oid_RSAEncryption : string
 let oid_RSAEncryption = ""
-val oid_SHAWithRSAEncryption : string
+
+abstract val oid_SHAWithRSAEncryption : string
 let oid_SHAWithRSAEncryption = ""
-val oid_SHA256WithRSAEncryption : string
+
+abstract val oid_SHA256WithRSAEncryption : string
 let oid_SHA256WithRSAEncryption = ""
-val oid_DSASignatureKey : string
+
+abstract val oid_DSASignatureKey : string
 let oid_DSASignatureKey = ""
 
-val oid_of_keyalg: sigAlg -> string
+abstract val oid_of_keyalg: sigAlg -> string
 let oid_of_keyalg salg = ""
 
-assume type X509Certificate2
+abstract new type X509Certificate2
 type hint = string
 type cert = b:bytes{length b < 65536}
 type chain = l:list cert{List.length l < 4}
 
-val x509_is_for_signing: X509Certificate2 -> bool
+abstract val x509_is_for_signing: X509Certificate2 -> bool
 let x509_is_for_signing x = failwith "Not implemented"
 
-val x509_verify: X509Certificate2 -> bool
+abstract val x509_verify: X509Certificate2 -> bool
 let x509_verify x = failwith "Not implemented"
 
-val x509_chain: X509Certificate2 -> list X509Certificate2
+abstract val x509_chain: X509Certificate2 -> list X509Certificate2
 let x509_chain x = failwith "Not implemented"
 
-val x509_check_key_sig_alg_one: list Sig.alg -> X509Certificate2 -> bool
+abstract val x509_check_key_sig_alg_one: list Sig.alg -> X509Certificate2 -> bool
 let x509_check_key_sig_alg_one l x = failwith "Not implemented"
 
-val x509_to_secret_key: X509Certificate2 -> option Sig.skey
-val x509_to_public_key: X509Certificate2 -> option Sig.pkey
+abstract val x509_to_secret_key: X509Certificate2 -> option Sig.skey
+abstract val x509_to_public_key: X509Certificate2 -> option Sig.pkey
 let x509_to_secret_key x = failwith "Not implemented"
 let x509_to_public_key x = failwith "Not implemented"
 
-val x509_is_for_key_encryption: X509Certificate2 -> bool
+abstract val x509_is_for_key_encryption: X509Certificate2 -> bool
 let x509_is_for_key_encryption x = failwith "Not implemented"
 
-val x509_export_public: X509Certificate2 -> bytes
+abstract val x509_export_public: X509Certificate2 -> bytes
 let x509_export_public x = failwith "Not implemented"
 
-val cert_to_x509: cert -> option X509Certificate2
+abstract val cert_to_x509: cert -> option X509Certificate2
 let cert_to_x509 c = failwith "Not implemented"
 
-val chain_to_x509list: chain -> option (list X509Certificate2)
+abstract val chain_to_x509list: chain -> option (list X509Certificate2)
 let chain_to_x509list c  = failwith "Not implemented"
 
-val x509list_to_chain: list X509Certificate2 -> chain
+abstract val x509list_to_chain: list X509Certificate2 -> chain
 let x509list_to_chain l = failwith "Not implemented"
 
 (* First argument (list Sig.alg>) gives the allowed signing alg. used for
  * signing the keys of the chain.
  *)
 
-val validate_x509_chain: list Sig.alg -> chain -> bool
+abstract val validate_x509_chain: list Sig.alg -> chain -> bool
 let validate_x509_chain l c  = failwith "Not implemented"
 
-val validate_x509list: X509Certificate2 -> list X509Certificate2 -> bool
+abstract val validate_x509list: X509Certificate2 -> list X509Certificate2 -> bool
 let validate_x509list x l = failwith "Not implemented"
 
-val is_for_signing:        cert -> bool
+abstract val is_for_signing:        cert -> bool
 let is_for_signing c = failwith "Not implemented"
-val is_for_key_encryption: cert -> bool
+abstract val is_for_key_encryption: cert -> bool
 let is_for_key_encryption c = failwith "Not implemented"
 
-val find_sigcert_and_alg: list Sig.alg -> hint -> list Sig.alg -> option (X509Certificate2 * Sig.alg)
+abstract val find_sigcert_and_alg: list Sig.alg -> hint -> list Sig.alg -> option (X509Certificate2 * Sig.alg)
 let find_sigcert_and_alg l h l2 = failwith "Not implemented"
 
-val find_enccert: list Sig.alg -> hint -> option X509Certificate2
+abstract val find_enccert: list Sig.alg -> hint -> option X509Certificate2
 let find_enccert l h = failwith "Not implemented"
 
-val get_chain_key_algorithm: chain -> option sigAlg
+abstract val get_chain_key_algorithm: chain -> option sigAlg
 let get_chain_key_algorithm c = failwith "Not implemented"
 
-val get_name_info: X509Certificate2 -> string
+abstract val get_name_info: X509Certificate2 -> string
 let get_name_info x = failwith "Not implemented"
