src/tls/Cert.fst
@@ -12,33 +12,40 @@ type chain = UntrustedCert.chain
 type sign_cert = option (chain * Sig.alg * Sig.skey)
 type enc_cert  = option (chain * RSAKey.sk)
 
-val for_signing : list Sig.alg -> hint -> list Sig.alg -> sign_cert
+
+abstract val for_signing : list Sig.alg -> hint -> list Sig.alg -> sign_cert
 let for_signing l h l2 = failwith "Not implemented"
-val for_key_encryption : list Sig.alg -> hint -> enc_cert
+
+abstract val for_key_encryption : list Sig.alg -> hint -> enc_cert
 let for_key_encryption l h = failwith "Not implemented"
 
-val get_public_signing_key : cert -> Sig.alg -> Result Sig.pkey
+abstract val get_public_signing_key : cert -> Sig.alg -> Result Sig.pkey
 let get_public_signing_key c a = failwith "Not implemented"
 
-val get_public_encryption_key : cert -> Result RSAKey.pk
+abstract val get_public_encryption_key : cert -> Result RSAKey.pk
 let get_public_encryption_key c = failwith "Not implemented"
 
-val get_chain_public_signing_key : chain -> Sig.alg -> Result Sig.pkey
-val get_chain_public_encryption_key : chain -> Result RSAKey.pk
+abstract val get_chain_public_signing_key : chain -> Sig.alg -> Result Sig.pkey
 let get_chain_public_signing_key c a = failwith "Not implemented"
+
+abstract val get_chain_public_encryption_key : chain -> Result RSAKey.pk
 let get_chain_public_encryption_key c = failwith "Not implemented"
 
-val is_chain_for_signing : chain -> bool
-val is_chain_for_key_encryption : chain -> bool
+abstract val is_chain_for_signing : chain -> bool
 let is_chain_for_signing c = failwith "Not implemented"
+
+abstract val is_chain_for_key_encryption : chain -> bool
 let is_chain_for_key_encryption c = failwith "Not implemented"
 
-val get_hint : chain -> option hint
-val validate_cert_chain : list Sig.alg  -> chain -> bool
-val parseCertificateList: bytes -> Result chain
-val certificateListBytes: chain -> Tot (b:bytes{length b < (3 * 65536)})
+abstract val get_hint : chain -> option hint
 let get_hint c = failwith "Not implemented"
+
+abstract val validate_cert_chain : list Sig.alg  -> chain -> bool
 let validate_cert_chain l c = failwith "Not implemented"
+
+abstract val parseCertificateList: bytes -> Result chain
 // Dummy implementation while certificate parsing is not implemented
 let parseCertificateList b = Correct ([b])
+
+abstract val certificateListBytes: chain -> Tot (b:bytes{length b < (3 * 65536)})
 let certificateListBytes c = magic()
